Checkpoint notes on many more bugs in etcd's leasing library;
leasingKV is somewhat challenging to salvage into something that seems
correct.

new/proof/go_etcd_io/etcd/client/v3/leasing_proof/protocol.v
@@ -2,8 +2,13 @@ Require Import New.proof.proof_prelude.
 
 Require Import New.proof.go_etcd_io.etcd.client.v3.
 
-(* FIXME: the original leasingkv has the following cache-consistency protocol
-   bug (see https://github.com/upamanyus/etcd/commit/174a964e806707b9fde186ade4b12be61967e9ea):
+(* NOTE(bug): the original leasingkv does not correctly check for lease expiration
+   when handling a Get(). *)
+
+(* NOTE(bug): Concurrent delete and puts with the same leasingKV are not handled
+   properly (permanent cache inconsistency).
+   `TestLeasingConcurrentPutDelete`
+   https://github.com/upamanyus/etcd/commit/174a964e806707b9fde186ade4b12be61967e9ea
 
    When Delete and Put run concurrently, if the server executes Put before
    Delete, but the cache processes the Delete response before the Put response,
@@ -19,9 +24,50 @@ Require Import New.proof.go_etcd_io.etcd.client.v3.
    check if (cacheResp.Header.Revision < respHeader.Revision), and only then
    update the cache. That's more like what leaseCache.Delete does.
 
-   This would give a cleaner definition to `is_newer_response` than is possible
-   now.
+   Solution: always use the response header revision number to decide whether to
+   overwrite the currently cached value.
  *)
+
+(* NOTE(bug): Concurrent Puts result in the version number temporarily being
+  incorrect. The client increments Version number every time a `leaseCache.Update`
+  happens, so if there were two concurrent Puts, there will be two increments.
+  However, it is possible that the Put with a higher ModRevision is incorporated
+  into the cache first, in which case its version number will temporarily be
+  `oldVer + 1` and will only become the correct value `oldVer + 2` after the
+  `leaseCache.Update` is called for the other Put.
+  Solution: use `prev_kv` to deduce the current version number.
+ *)
+
+(* NOTE(bug): pretty sure Txns don't work correctly w.r.t concurrent Gets
+   because they don't use waitc. Didn't set up a failing test case to confirm
+   this. Just deleted the Txn implementation and tests. *)
+
+
+(* NOTE(bug): Concurrent Get and Put on the same leasingKV can result in the Get
+   returning stale information if the Put RPC doesn't get a response from the
+   server, because it would evict the leaseEntry from the entries and close waitc.
+   The Get() call would just read whatever was in the cache before. This could
+   probably be triggered if the key got evicted during a Put() for other reasons
+   too (e.g. a different client causing it to get revoked).
+  `TestLeasingConcurrentPutGet`
+   https://github.com/upamanyus/etcd/commit/e11ce2ae7d90f482814ff1a1f851179d36ff419f
+   Possible solution: if key gets evicted from our cache somehow while doing the
+   Put, then signal to any outstanding Get() call that the key is not cached.
+*)
+
+(* NOTE(bug): Two concurrent Puts can result in the cache being marked as "ok to
+   read" even though one of the Puts is still in progress. Can try to create a
+   failing test by getting Puts to linearize in the opposite order of their
+   waitcs.
+   Possible solution: get waitcs for all pending Puts for the key, and wait for them all
+   to successfully finish before reading the cached value and returning.
+ *)
+
+(* NOTE(bug): Puts are not at-most-once. If the first Put RPC's response from
+   the server is dropped, then the client will just make another Put RPC. So,
+   e.g., the version number can increase by an arbitrary amount.
+   Possible solution: distinguish a PutRPC error from a "Txn Succeeded == false" response.
+*)
 
 (* To simplify the proof for now, assuming that all keys are managed by
    leasingKV clients (i.e. the whole map is subject to the following
@@ -30,14 +76,16 @@ Require Import New.proof.go_etcd_io.etcd.client.v3.
    The key being modified by `Put` must not have prefix `pfx`.
  *)
 
+(*
 Section protocol.
 
 Context {W : Type} {W_eq_dec : EqDecision W} {W_countable : Countable W}.
 
-Inductive LeasedValue :=
-| LeasedValuePresent (lv_mod_rev : Z) (lv_val : go_string)
-| LeasedValueDeleted (lv_del_rev : Z)
-.
+Record LeasedValue :=
+  {
+    lv_rev : Z;
+    lv_val : option go_string
+  }.
 
 Record LeasedEntry :=
   {
@@ -71,13 +119,16 @@ Global Instance settable_CacheState : Settable CacheState :=
 Context `{!invGS Σ}.
 
 Definition own_server_inv (γs : ServerNames) (s : EtcdState.t) : iProp Σ.
-Admitted.
+Proof. Admitted.
 
 Definition own_cache_inv (γc : CacheNames) (c : CacheState) : iProp Σ.
-Admitted.
+Proof. Admitted.
 
-Definition own_Locked (w : W) (rev : Z) : iProp Σ.
-Admitted.
+Definition own_Locked (w : W) : iProp Σ.
+Proof. Admitted.
+
+Definition own_CanPut (w : W) (rev : Z) : iProp Σ.
+Proof. Admitted.
 
 Context (c c' : CacheState).
 Context (s s' : EtcdState.t).
@@ -95,7 +146,8 @@ Lemma take_step_Lock (key : go_string) w rev :
   step_Lock key w rev →
   own_cache_inv γc c ==∗
   own_cache_inv γc c' ∗
-  own_Locked w rev.
+  own_Locked w ∗
+  own_Update rev.
 Proof.
 Admitted.
 
@@ -126,14 +178,21 @@ Lemma take_step_Evict key w rev :
 Proof.
 Admitted.
 
-(* FIXME: need ResponseHeader. *)
 Definition is_newer_response (lv : LeasedValue) (resp_rev : Z) : Prop :=
-  True.
+  lv.(lv_rev) ≤ resp_rev.
 
 Definition step_Update key val resp_rev : Prop :=
   ∃ le,
   c.(entries) !! key = Some le ∧
   is_newer_response le.(le_value) resp_rev ∧
-  c' = c <| entries := <[ key := le <| le_value := LeasedValuePresent resp_rev val |> ]> c.(entries) |>.
+  c' = c <| entries := <[ key := le <| le_value := {| lv_rev := resp_rev; lv_val := val |} |> ]> c.(entries) |>.
 
-End protocol.
+Lemma take_step_Update key val resp_rev w rev :
+  step_Update key val resp_rev →
+  own_Locked w rev -∗
+  own_cache_inv γs c ==∗
+  own_cache_inv γs c'.
+
+Definition close :
+
+End protocol. *)
